---
title: The keep-change-flip rule for fractions
description: This proof shows the famous keep-change-flip rule when dividing by fractions.
category: algebra
---

## Statement

When dividing by a fraction, you multiply by the reciprocal.

$$ a \div \frac{b}{c} = a \* \frac{c}{b} $$

## Proof

Write the fraction using negative exponents.

$$ a \div \frac{b}{c} = a \div (b \* c^{-1}) $$

Now write the division using negative exponents as well.

$$ a \div \frac{b}{c} = a \* (b \* c^{-1})^{-1} $$

Append the powers to the factors.

$$ a \div \frac{b}{c} = a \* b^{-1} \* (c^{-1})^{-1} $$

Multiply the exponents.

$$ a \div \frac{b}{c} = a \* b^{-1} \* c^1 $$

Finally, write $ b^{-1} \* c $ as a fraction again.

$$ a \div \frac{b}{c} = a \* \frac{c}{b} $$
